\documentclass[11pt,letterpaper]{article}
\usepackage[english]{babel}
\usepackage{amsfonts}
\usepackage{amssymb}
\usepackage{amsmath}
\pagestyle{empty}
\textwidth = 16.5 cm
\textheight = 24.5 cm
\oddsidemargin = 0.0 cm
\evensidemargin = 0.0 cm
\topmargin = 0.0 cm
\headheight = 0.0 cm
\headsep = 0.0 cm 
\date{}

\title{Useful Identities in Quantum Optics}
\author{Nicol\'as Quesada\\{\small \sf Instituto de F\'isica, Universidad de Antioquia}}

\begin{document}
\maketitle
\thispagestyle{empty}

\subsection*{Notation}
Latin letters with caret ($\hat a, \hat x, \hat y, \hat z$) denote linear operators.\\
Greek letters ($\alpha, \lambda$) denote $\mathbb{C}$ numbers.\\
The hermitian adjoint of $\hat a$ is denoted $\hat a^{\dagger}$.\\
The commutator of two operators $\hat x$ and $\hat y$ is defined as:
$ [\hat x,\hat y] := \hat x \hat y-\hat y \hat x$ \\

\subsection*{Leibniz's law }
$$ [\hat x, \hat y \hat z]=[\hat x, \hat y] \hat z+\hat y[\hat x,\hat z] $$
$$ [\hat x \hat y, \hat z]=[\hat x, \hat z] \hat y+\hat x[\hat y,\hat z] $$

\subsection*{Jacobi Identity}
$$ [\hat x, [ \hat y, \hat z]]+[ \hat y,[ \hat z,\hat x]]+[\hat z, [\hat x, \hat y]]=0 $$
\subsection*{Baker-Campbell-Hausdorff formula}
If $[\hat x,[\hat x,\hat y]]=[\hat y,[\hat x,\hat y]]=0$ then:
$$e^{\hat x+\hat y}=\exp{\left(-\frac{1}{2} [\hat x,\hat y] \right)} e^{\hat x} e^{\hat y}=\exp{\left(\frac{1}{2} [\hat x,\hat y] \right)} e^{\hat y} e^{\hat x} $$

\subsection*{Hadamard lemma}
$$ e^{ i \lambda \hat x} \hat y e^{- i \lambda \hat x}=\hat y + i \lambda [\hat x,\hat y]+\frac{(i \lambda)^2}{2!}[\hat x,[\hat x,\hat y]]+\ldots$$

\subsection*{Identities for Bosonic Operators}
The bosonic operators $\hat a$ and $\hat a^\dagger$ satisfy $[\hat a,\hat a^\dagger]=\hat 1$
$$[\hat a,f(\hat a,\hat a^\dagger)]=\frac{\partial f}{\partial \hat a^\dagger}$$
$$[\hat a^\dagger,f(\hat a,\hat a^\dagger)]=-\frac{\partial f}{\partial \hat a}$$
$$e^{-\alpha \hat a^\dagger \hat a} f(\hat a,\hat a^\dagger) e^{\alpha \hat a^\dagger \hat a}=f(\hat a e^\alpha,\hat a^\dagger e^{-\alpha})$$

\begin{thebibliography}{}
\bibitem{} J.J. Sakurai, \textit{Modern Quantum Mechanics}, Addison Wesley Longman
\bibitem{} M.O. Scully, M.S. Zubairy \textit{Quantum Optics}, Cambridge University Press.
\end{thebibliography}


\end{document}

